src/MemInjProps.v
@@ -2,6 +2,9 @@ Require Import compcert.common.Values.
 Require Import compcert.common.Memory.
 Require Import compcert.common.Globalenvs.
 
+Require Import oeuf.StuartTact.
+Require Import StructTact.StructTactics.
+
 Require Import ZArith.
 
 Local Open Scope Z_scope.
@@ -19,3 +22,6 @@ Definition globals_inj_same {F V} (ge : Genv.t F V) (mi : meminj) : Prop :=
     (Genv.find_funct_ptr ge b = Some f \/
     Genv.find_var_info ge b = Some v) ->
     mi b = Some (b,0).
+
+Definition inject_ext mi b b' : positive -> option (positive * Z) :=
+    fun x => if Pos.eq_dec x b then Some (b', 0) else mi x.
